tll session

coq_session/dyn_subst.v
@@ -6,104 +6,197 @@ Set Implicit Arguments.
 Unset Strict Implicit.
 Unset Printing Implicit Defensive.
 
-Reserved Notation "Γ1 ; Δ1 ⊢ σ ⊣ Γ2 ; Δ2" (at level 50, Δ1, σ, Γ2 at next level).
+Reserved Notation "Θ1 ; Γ1 ; Δ1 ⊢ σ ⊣ Γ2 ; Δ2"
+  (at level 50, Γ1, Δ1, σ, Γ2, Δ2 at next level).
 Inductive dyn_agree_subst :
-  sta_ctx -> dyn_ctx -> (var -> term) -> sta_ctx -> dyn_ctx -> Prop :=
-| dyn_agree_subst_nil σ :
-  nil ; nil ⊢ σ ⊣ nil ; nil
-| dyn_agree_subst_ty Γ1 Δ1 σ Γ2 Δ2 A s :
-  Γ1 ; Δ1 ⊢ σ ⊣ Γ2 ; Δ2 ->
+  dyn_ctx -> sta_ctx -> dyn_ctx -> (var -> term) -> sta_ctx -> dyn_ctx -> Prop :=
+| dyn_agree_subst_nil Θ1 :
+  dyn_empty Θ1 ->
+  Θ1 ; nil ; nil ⊢ ids ⊣ nil ; nil
+| dyn_agree_subst_ty Θ1 Γ1 Δ1 σ Γ2 Δ2 A s :
+  Θ1 ; Γ1 ; Δ1 ⊢ σ ⊣ Γ2 ; Δ2 ->
   Γ2 ⊢ A : Sort s ->
-  (A.[σ] :: Γ1) ; (A.[σ] :{s} Δ1) ⊢ up σ ⊣ (A :: Γ2) ; (A :{s} Δ2)
-| dyn_agree_subst_n Γ1 Δ1 σ Γ2 Δ2 A s :
-  Γ1 ; Δ1 ⊢ σ ⊣ Γ2 ; Δ2 ->
+  Θ1 ; (A.[σ] :: Γ1) ; (A.[σ] :{s} Δ1) ⊢ up σ ⊣ (A :: Γ2) ; (A :{s} Δ2)
+| dyn_agree_subst_n Θ1 Γ1 Δ1 σ Γ2 Δ2 A s :
+  Θ1 ; Γ1 ; Δ1 ⊢ σ ⊣ Γ2 ; Δ2 ->
   Γ2 ⊢ A : Sort s ->
-  (A.[σ] :: Γ1) ; (_: Δ1) ⊢ up σ ⊣ (A :: Γ2) ; (_: Δ2)
-| dyn_agree_subst_wk0 Γ1 Δ1 σ Γ2 Δ2 n A :
-  Γ1 ; Δ1 ⊢ σ ⊣ Γ2 ; Δ2 ->
+  Θ1 ; (A.[σ] :: Γ1) ; (_: Δ1) ⊢ up σ ⊣ (A :: Γ2) ; (_: Δ2)
+| dyn_agree_subst_wk0 Θ1 Γ1 Δ1 σ Γ2 Δ2 n A :
+  Θ1 ; Γ1 ; Δ1 ⊢ σ ⊣ Γ2 ; Δ2 ->
   Γ1 ⊢ n : A.[σ] ->
-  Γ1 ; Δ1 ⊢ n .: σ ⊣ (A :: Γ2) ; (_: Δ2)
-| dyn_agree_subst_wk1 Γ1 Γ2 σ Δ1 Δ2 Δa Δb n A s :
+  Θ1 ; Γ1 ; Δ1 ⊢ n .: σ ⊣ (A :: Γ2) ; (_: Δ2)
+| dyn_agree_subst_wk1 Θa Θb Θ1 Γ1 Γ2 σ Δ1 Δ2 Δa Δb n A s :
+  Θb ▷ s ->
   Δb ▷ s ->
+  Θa ∘ Θb => Θ1 ->
   Δa ∘ Δb => Δ1 ->
-  Γ1 ; Δa ⊢ σ ⊣ Γ2 ; Δ2 ->
-  Γ1 ; Δb ⊢ n : A.[σ] ->
-  Γ1 ; Δ1 ⊢ n .: σ ⊣ (A :: Γ2) ; (A :{s} Δ2)
-| dyn_agree_subst_conv0 Γ1 Δ1 σ Γ2 Δ2 A B s :
+  Θa ; Γ1 ; Δa ⊢ σ ⊣ Γ2 ; Δ2 ->
+  Θb ; Γ1 ; Δb ⊢ n : A.[σ] ->
+  Θ1 ; Γ1 ; Δ1 ⊢ n .: σ ⊣ (A :: Γ2) ; (A :{s} Δ2)
+| dyn_agree_subst_conv0 Θ1 Γ1 Δ1 σ Γ2 Δ2 A B s :
   A === B ->
   Γ1 ⊢ B.[ren (+1)].[σ] : Sort s ->
   Γ2 ⊢ B : Sort s ->
-  Γ1 ; Δ1 ⊢ σ ⊣ (A :: Γ2) ; (_: Δ2) ->
-  Γ1 ; Δ1 ⊢ σ ⊣ (B :: Γ2) ; (_: Δ2)
-| dyn_agree_subst_conv1 Γ1 Δ1 σ Γ2 Δ2 A B s :
+  Θ1 ; Γ1 ; Δ1 ⊢ σ ⊣ (A :: Γ2) ; (_: Δ2) ->
+  Θ1 ; Γ1 ; Δ1 ⊢ σ ⊣ (B :: Γ2) ; (_: Δ2)
+| dyn_agree_subst_conv1 Θ1 Γ1 Δ1 σ Γ2 Δ2 A B s :
   A === B ->
   Γ1 ⊢ B.[ren (+1)].[σ] : Sort s ->
   Γ2 ⊢ B : Sort s ->
-  Γ1 ; Δ1 ⊢ σ ⊣ (A :: Γ2) ; (A :{s} Δ2) ->
-  Γ1 ; Δ1 ⊢ σ ⊣ (B :: Γ2) ; (B :{s} Δ2)
-where "Γ1 ; Δ1 ⊢ σ ⊣ Γ2 ; Δ2" := (dyn_agree_subst Γ1 Δ1 σ Γ2 Δ2).
+  Θ1 ; Γ1 ; Δ1 ⊢ σ ⊣ (A :: Γ2) ; (A :{s} Δ2) ->
+  Θ1 ; Γ1 ; Δ1 ⊢ σ ⊣ (B :: Γ2) ; (B :{s} Δ2)
+where "Θ1 ; Γ1 ; Δ1 ⊢ σ ⊣ Γ2 ; Δ2" := (dyn_agree_subst Θ1 Γ1 Δ1 σ Γ2 Δ2).
 
-Lemma dyn_agree_subst_key Γ1 Γ2 Δ1 Δ2 σ s :
-  Γ1 ; Δ1 ⊢ σ ⊣ Γ2 ; Δ2 -> Δ2 ▷ s -> Δ1 ▷ s.
-Proof with eauto using key.
-  move=>agr. elim: agr s=>{Γ1 Γ2 Δ1 Δ2 σ}...
-  { move=>Γ1 Δ1 σ Γ2 Δ2 A s agr ih tyA r k. inv k... }
-  { move=>Γ1 Δ1 σ Γ2 Δ2 A s agr ih tyA r k. inv k... }
-  { move=>Γ1 Δ1 σ Γ2 Δ2 n A agr ih tyn s k. inv k... }
-  { move=>Γ1 Γ2 σ Δ1 Δ2 Δa Δb n A s k1 mrg agr ih tyn r k2. inv k2...
-    apply: key_merge...
-    apply: key_impure. }
-  { move=>Γ1 Δ1 σ Γ2 Δ2 A B s eq tyB1 tyB2 agr ih r k. inv k... }
+Lemma dyn_agree_subst_key Θ1 Γ1 Γ2 Δ1 Δ2 σ s :
+  Θ1 ; Γ1 ; Δ1 ⊢ σ ⊣ Γ2 ; Δ2 -> Δ2 ▷ s -> Θ1 ▷ s /\ Δ1 ▷ s.
+Proof with eauto using key, key_empty, key_merge, key_impure.
+  move=>agr. elim: agr s=>{Θ1 Γ1 Γ2 Δ1 Δ2 σ}...
+  { move=>Θ1 Γ1 Δ1 σ Γ2 Δ2 A s agr ih tyA r k. inv k... have[]:=ih _ H3... }
+  { move=>Θ1 Γ1 Δ1 σ Γ2 Δ2 A s agr ih tyA r k. inv k... have[]:=ih _ H0... }
+  { move=>Θ1 Γ1 Δ1 σ Γ2 Δ2 n A agr ih tyn s k. inv k... }
+  { move=>Θa Θb Θ1 Γ1 Γ2 σ Δ1 Δ2 Δa Δb n A s k1 k2 mrg1 mrg2 agr ih tyn r k3. inv k3...
+    have[]:=ih _ H3... }
+  { move=>Θ1 Γ1 Δ1 σ Γ2 Δ2 A B s eq tyB1 tyB2 agr ih r k. inv k... }
 Qed.
 
-Lemma dyn_sta_agree_subst Γ1 Γ2 Δ1 Δ2 σ :
-  Γ1 ; Δ1 ⊢ σ ⊣ Γ2 ; Δ2 -> Γ1 ⊢ σ ⊣ Γ2.
+Lemma dyn_sta_agree_subst Θ1 Γ1 Γ2 Δ1 Δ2 σ :
+  Θ1 ; Γ1 ; Δ1 ⊢ σ ⊣ Γ2 ; Δ2 -> Γ1 ⊢ σ ⊣ Γ2.
 Proof with eauto using sta_agree_subst.
-  elim=>{Γ1 Γ2 Δ1 Δ2 σ}...
-  move=>Γ1 Γ2 σ Δ1 Δ2 Δa Δb n A s _ _ _ agr tyn.
+  elim=>{Θ1 Γ1 Γ2 Δ1 Δ2 σ}...
+  move=>Θa Θb Θ1 Γ1 Γ2 σ Δ1 Δ2 Δa Δb n A s _ _ _ _ agr ih tyn.
   constructor...
   apply: dyn_sta_type...
 Qed.
 
-Lemma dyn_agree_subst_refl Γ Δ : dyn_wf Γ Δ -> Γ ; Δ ⊢ ids ⊣ Γ ; Δ.
+Lemma dyn_agree_subst_refl Θ Γ Δ :
+  dyn_empty Θ -> dyn_wf Γ Δ -> Θ ; Γ ; Δ ⊢ ids ⊣ Γ ; Δ.
 Proof with eauto using dyn_agree_subst.
-  elim: Γ Δ.
-  { move=>Δ wf. inv wf... }
-  { move=>A Γ ih Δ wf. inv wf.
-    { have agr:=ih _ H1.
-      have:(A.[ids] :: Γ); A.[ids] :{s} Δ0 ⊢ up ids ⊣ (A :: Γ); A :{s} Δ0...
+  elim: Γ Θ Δ.
+  { move=>Θ Δ emp wf. inv wf... }
+  { move=>A Γ ih Θ Δ emp wf. inv wf.
+    { have agr:=ih Θ _ emp H1.
+      have:Θ ; (A.[ids] :: Γ); A.[ids] :{s} Δ0 ⊢ up ids ⊣ (A :: Γ); A :{s} Δ0...
       by asimpl. }
-    { have agr:=ih _ H1.
-      have:(A.[ids] :: Γ); _: Δ0 ⊢ up ids ⊣ (A :: Γ); _: Δ0...
+    { have agr:=ih Θ _ emp H1.
+      have:Θ ; (A.[ids] :: Γ); _: Δ0 ⊢ up ids ⊣ (A :: Γ); _: Δ0...
       by asimpl. } }
 Qed.
 Hint Resolve dyn_agree_subst_refl.
 
-Lemma dyn_agree_subst_has Γ1 Γ2 σ Δ1 Δ2 x s A :
-  Γ1 ; Δ1 ⊢ σ ⊣ Γ2 ; Δ2 -> dyn_wf Γ1 Δ1 -> dyn_has Δ2 x s A -> Γ1 ; Δ1 ⊢ (σ x) : A.[σ].
+Lemma dyn_type_empty Θ1 Γ Δ m A :
+  Θ1 ; Γ ; Δ ⊢ m : A -> exists Θ, dyn_empty Θ /\ Θ ∘ Θ1 => Θ1.
+Proof with eauto using dyn_type, key_empty.
+  move=>ty. elim: ty=>{Θ1 Γ Δ m A}...
+  { move=>Θ Γ Δ x s A emp wf shs dhs. exists Θ. split... apply: empty_merge_self... }
+  { move=>Θ1 Θ2 Θ Γ Δ1 Δ2 Δ A B m n s mrg1 mrg2 tym[Θm[empm mrgm]]tyn[Θn[empn mrgn]].
+    have[Θx[Θy[mrgx[mrgy mrgz]]]]:=merge_distr mrg1 mrgm mrgn.
+    have e:=merge_inj mrg1 mrgz. subst.
+    exists Θx. split... apply: merge_empty... }
+  { move=>Θ1 Θ2 Θ Γ Δ1 Δ2 Δ A B m n t mrg1 mrg2 tyS tym[Θm[empm mrgm]]tyn[Θn[empn mrgn]].
+    have[Θx[Θy[mrgx[mrgy mrgz]]]]:=merge_distr mrg1 mrgm mrgn.
+    have e:=merge_inj mrg1 mrgz. subst.
+    exists Θx. split... apply: merge_empty... }
+  { move=>Θ1 Θ2 Θ Γ Δ1 Δ2 Δ A B C m n s r t mrg1 mrg2 tyC tym[Θm[empm mrgm]]tyn[Θn[empn mrgn]].
+    have[Θx[Θy[mrgx[mrgy mrgz]]]]:=merge_distr mrg1 mrgm mrgn.
+    have e:=merge_inj mrg1 mrgz. subst.
+    exists Θx. split... apply: merge_empty... }
+  { move=>Θ1 Θ2 Θ Γ Δ1 Δ2 Δ A B C m n s r1 r2 t mrg1 mrg2 tyC tym[Θm[empm mrgm]]tyn[Θn[empn mrgn]].
+    have[Θx[Θy[mrgx[mrgy mrgz]]]]:=merge_distr mrg1 mrgm mrgn.
+    have e:=merge_inj mrg1 mrgz. subst.
+    exists Θx. split... apply: merge_empty... }
+  { move=>Θ Γ Δ emp wf k. exists Θ. split... apply: empty_merge_self... }
+  { move=>Θ Γ Δ emp wf k. exists Θ. split... apply: empty_merge_self... }
+  { move=>Θ Γ Δ emp wf k. exists Θ. split... apply: empty_merge_self... }
+  { move=>Θ1 Θ2 Θ Γ Δ1 Δ2 Δ A m n1 n2 s mrg1 mrg2 tyA
+     tym[Θm[empm mrgm]]tyn1[Θn1[empn1 mrgn1]]tyn2[Θn2[empn2 mrgn2]].
+    have[Θx[Θy[mrgx[mrgy mrgz]]]]:=merge_distr mrg1 mrgm mrgn1.
+    have e:=merge_inj mrg1 mrgz. subst.
+    exists Θx. split... apply: merge_empty... }
+  { move=>Θ1 Θ2 Θ Γ Δ1 Δ2 Δ m n A B s t mrg1 mrg2 tyB tym[Θm[empm mrgm]]tyn[Θn[empn mrgn]].
+    have[Θx[Θy[mrgx[mrgy mrgz]]]]:=merge_distr mrg1 mrgm mrgn.
+    have e:=merge_inj mrg1 mrgz. subst.
+    exists Θx. split... apply: merge_empty... }
+  { move=>Θ Γ Δ r x A js wf k tyA. apply: just_empty... }
+Qed.
+
+
+(* Lemma dyn_type_empty Θ1 Θ2 Γ Δ m A : *)
+(*   Θ1 ; Γ ; Δ ⊢ m : A -> dyn_empty Θ1 -> dyn_empty Θ2 -> Θ2 ; Γ ; Δ ⊢ m : A. *)
+(* Proof with eauto using dyn_type, key_empty. *)
+(*   move=>ty. elim: ty Θ2=>{Θ1 Γ Δ m A}... *)
+(*   { move=>Θ1 Θ2 Θ Γ Δ1 Δ2 Δ A B m n s mrg1 mrg2 tym ihm tyn ihn Θ3 emp emp3. *)
+(*     have[emp1 emp2]:=empty_split mrg1 emp. *)
+(*     have{}ihm:=ihm _ emp1 emp3. *)
+(*     have{}ihn:=ihn _ emp2 emp3. *)
+(*     apply: dyn_app1... *)
+(*     apply: empty_merge_self... } *)
+(*   { move=>Θ1 Θ2 Θ Γ Δ1 Δ2 Δ A B m n t mrg1 mrg2 tyS tym ihm tyn ihn Θ3 emp emp3. *)
+(*     have[emp1 emp2]:=empty_split mrg1 emp. *)
+(*     have{}ihm:=ihm _ emp1 emp3. *)
+(*     have{}ihn:=ihn _ emp2 emp3. *)
+(*     apply: dyn_pair1... *)
+(*     apply: empty_merge_self... } *)
+(*  { move=>Θ1 Θ2 Θ Γ Δ1 Δ2 Δ A B C m n s r t mrg1 mrg2 tyS tym ihm tyn ihn Θ3 emp emp3. *)
+(*     have[emp1 emp2]:=empty_split mrg1 emp. *)
+(*     have{}ihm:=ihm _ emp1 emp3. *)
+(*     have{}ihn:=ihn _ emp2 emp3. *)
+(*     apply: dyn_letin0... *)
+(*     apply: empty_merge_self... } *)
+(*  { move=>Θ1 Θ2 Θ Γ Δ1 Δ2 Δ A B C m n s r1 r2 t mrg1 mrg2 tyS tym ihm tyn ihn Θ3 emp emp3. *)
+(*     have[emp1 emp2]:=empty_split mrg1 emp. *)
+(*     have{}ihm:=ihm _ emp1 emp3. *)
+(*     have{}ihn:=ihn _ emp2 emp3. *)
+(*     apply: dyn_letin1... *)
+(*     apply: empty_merge_self... } *)
+(*  { move=>Θ1 Θ2 Θ Γ Δ1 Δ2 Δ A m n1 n2 s mrg1 mrg2 tyA tym ihm tyn1 ihn1 tyn2 ihn2 Θ3 emp emp3. *)
+(*     have[emp1 emp2]:=empty_split mrg1 emp. *)
+(*     have{}ihm:=ihm _ emp1 emp3. *)
+(*     have{}ihn1:=ihn1 _ emp2 emp3. *)
+(*     have{}ihn2:=ihn2 _ emp2 emp3. *)
+(*     apply: dyn_ifte... *)
+(*     apply: empty_merge_self... } *)
+(*  { move=>Θ1 Θ2 Θ Γ Δ1 Δ2 Δ m n A B s t mrg1 mrg2 tyA tym ihm tyn ihn Θ3 emp emp3. *)
+(*     have[emp1 emp2]:=empty_split mrg1 emp. *)
+(*     have{}ihm:=ihm _ emp1 emp3. *)
+(*     have{}ihn:=ihn _ emp2 emp3. *)
+(*     apply: dyn_bind... *)
+(*     apply: empty_merge_self... } *)
+(*  { move=>Θ Γ Δ r x A js wf k tyA Θ2 emp. *)
+(*    exfalso. apply: empty_just... } *)
+(* Qed. *)
+  
+Lemma dyn_agree_subst_has Θ1 Θ2 Θ Γ1 Γ2 σ Δ1 Δ2 x s A :
+  Θ1 ; Γ1 ; Δ1 ⊢ σ ⊣ Γ2 ; Δ2 -> dyn_empty Θ2 -> Θ1 ∘ Θ2 => Θ ->
+  dyn_wf Γ1 Δ1 -> dyn_has Δ2 x s A -> Θ ; Γ1 ; Δ1 ⊢ (σ x) : A.[σ].
 Proof with eauto using dyn_agree_subst, dyn_agree_subst_key.
-  move=>agr. elim: agr x s A=>{Γ1 Γ2 σ Δ1 Δ2}...
-  { move=>σ x s A wf hs. inv hs. }
-  { move=>Γ1 Δ1 σ Γ2 Δ2 A s agr ih tyA x t B wf hs.
+  move=>agr. elim: agr x Θ2 Θ s A=>{Θ1 Γ1 Γ2 σ Δ1 Δ2}...
+  { move=>Θ1 emp1 x Θ2 Θ s A emp2 mrg wf hs. inv hs. }
+  { move=>Θ1 Γ1 Δ1 σ Γ2 Δ2 A s agr ih tyA x Θ2 Θ r B emp2 mrg wf hs.
     inv wf. inv hs; asimpl.
-    replace A.[σ >> ren (+1)] with A.[σ].[ren (+1)] by autosubst.
-    apply: dyn_var; constructor...
-    replace A0.[σ >> ren (+1)] with A0.[σ].[ren (+1)] by autosubst.
-    apply: dyn_eweakenU... }
-  { move=>Γ1 Δ1 σ Γ2 Δ2 A s agr ih tyA x t B wf hs.
+    { replace A.[σ >> ren (+1)] with A.[σ].[ren (+1)] by autosubst.
+      have[k1 k2]:=dyn_agree_subst_key agr H7.
+      apply: dyn_var.
+      have e:=merge_pureL mrg k1. subst...
+      constructor...
+      constructor...
+      constructor... }
+    { replace A0.[σ >> ren (+1)] with A0.[σ].[ren (+1)] by autosubst.
+      apply: dyn_eweakenU... } }
+  { move=>Θ1 Γ1 Δ1 σ Γ2 Δ2 A s agr ih tyA x Θ2 Θ t B emp mrg wf hs.
     inv wf. inv hs; asimpl...
-    replace A0.[σ >> ren (+1)] with A0.[σ].[ren (+1)]
-      by autosubst.
+    replace A0.[σ >> ren (+1)] with A0.[σ].[ren (+1)] by autosubst.
     apply: dyn_eweakenN... }
-  { move=>Γ1 Δ1 σ Γ2 Δ2 n A agr ih tyn x s B wf hs. inv hs; asimpl... }
-  { move=>Γ1 Γ2 σ Δ1 Δ2 Δa Δb n A s k mrg agr ih tyn x t B wf hs.
+  { move=>Θ1 Γ1 Δ1 σ Γ2 Δ2 n A agr ih tyn x Θ2 Θ s B emp mrg wf hs. inv hs; asimpl... }
+  { move=>Θa Θb Θ1 Γ1 Γ2 σ Δ1 Δ2 Δa Δb n A s k1 k2 mrg1 mrg2 agr ih tyn x Θ2 Θ t B emp mrg wf hs.
     inv hs; asimpl.
-    { have ka:=dyn_agree_subst_key agr H5.
-      have->//:=merge_pureL mrg ka. }
-    { have->:=merge_pureR mrg k.
-      apply: ih...
-      have[]//:=dyn_wf_inv mrg wf. } }
-  { move=>Γ1 Δ1 σ Γ2 Δ2 A B s eq tyB1 tyB2 agr ih x t C wf hs. inv hs.
+    { have[k3 k4]:=dyn_agree_subst_key agr H5.
+      have e:=merge_pureL mrg1 k3. subst.
+      have e:=merge_pureL mrg2 k4. subst.
+      have e:=merge_emptyR mrg emp. subst... }
+    { have e:=merge_pureR mrg1 k1. subst.
+      have e:=merge_pureR mrg2 k2. subst.
+      apply: ih... } }
+  { move=>Θ1 Γ1 Δ1 σ Γ2 Δ2 A B s eq tyB1 tyB2 agr ih x Θ2 Θ t C emp mrg wf hs. inv hs.
     { apply: dyn_conv.
       apply: sta_conv_subst.
       apply: sta_conv_subst...
@@ -114,169 +207,195 @@ Proof with eauto using dyn_agree_subst, dyn_agree_subst_key.
       constructor... } }
 Qed.
 
-Lemma dyn_agree_subst_merge Γ1 Γ2 Δ1 Δ2 Δa Δb σ :
-  Γ1 ; Δ1 ⊢ σ ⊣ Γ2 ; Δ2 -> Δa ∘ Δb => Δ2 ->
-  exists Δa' Δb',
-    Δa' ∘ Δb' => Δ1 /\ Γ1 ; Δa' ⊢ σ ⊣ Γ2 ; Δa /\ Γ1 ; Δb' ⊢ σ ⊣ Γ2 ; Δb.
+Lemma dyn_agree_subst_merge Θ1 Γ1 Γ2 Δ1 Δ2 Δa Δb σ :
+  Θ1 ; Γ1 ; Δ1 ⊢ σ ⊣ Γ2 ; Δ2 -> Δa ∘ Δb => Δ2 ->
+  exists Θa' Θb' Δa' Δb',
+    Θa' ∘ Θb' => Θ1 /\
+    Δa' ∘ Δb' => Δ1 /\
+    Θa' ; Γ1 ; Δa' ⊢ σ ⊣ Γ2 ; Δa /\
+    Θb' ; Γ1 ; Δb' ⊢ σ ⊣ Γ2 ; Δb.
 Proof with eauto 6 using merge, dyn_agree_subst, dyn_agree_subst_key.
-  move=>agr. elim: agr Δa Δb=>{Γ1 Γ2 Δ1 Δ2 σ}.
-  { move=>σ Δa Δb mrg. inv mrg.
-    exists nil. exists nil... }
-  { move=>Γ1 Δ1 σ Γ2 Δ2 A s agr ih tyA Δa Δb mrg. inv mrg.
-    { have[Δa[Δb[mrg[agra agrb]]]]:=ih _ _ H2.
-      exists (A.[σ] :U Δa). exists (A.[σ] :U Δb)... }
-    { have[Δa[Δb[mrg[agra agrb]]]]:=ih _ _ H2.
-      exists (A.[σ] :L Δa). exists (_: Δb)... }
-    { have[Δa[Δb[mrg[agra agrb]]]]:=ih _ _ H2.
-      exists (_: Δa). exists (A.[σ] :L Δb)... } }
-  { move=>Γ1 Δ1 σ Γ2 Δ2 A s agr ih tyA Δa Δb mrg. inv mrg.
-    have[Δa[Δb[mrg[agra agrb]]]]:=ih _ _ H2.
-    exists (_: Δa). exists (_: Δb)... }
-  { move=>Γ1 Δ1 σ Γ2 Δ2 n A agr ih tyn Δa Δb mrg. inv mrg.
-    have[Δa[Δb[mrg[agra agrb]]]]:=ih _ _ H2.
-    exists Δa. exists Δb... }
-  { move=>Γ1 Γ2 σ Δ1 Δ2 Δa Δb n A s k mrg agr ih tyn Δa' Δb' mrg'. inv mrg'.
-    { have[Δa'[Δb'[mrg'[agra agrb]]]]:=ih _ _ H2.
-      have[Δc[mrg1 mrg2]]:=merge_splitL mrg mrg'.
-      exists Δc. exists Δb'.
+  move=>agr. elim: agr Δa Δb=>{Θ1 Γ1 Γ2 Δ1 Δ2 σ}.
+  { move=>Θ1 emp Δa Δb mrg. inv mrg.
+    exists Θ1. exists Θ1. exists nil. exists nil. repeat split... apply: empty_merge_self... }
+  { move=>Θ1 Γ1 Δ1 σ Γ2 Δ2 A s agr ih tyA Δa Δb mrg. inv mrg.
+    { have[Θa[Θb[Δa[Δb[mrg1[mrg2[agra agrb]]]]]]]:=ih _ _ H2.
+      exists Θa. exists Θb. exists (A.[σ] :U Δa). exists (A.[σ] :U Δb).
+      repeat split... }
+    { have[Θa[Θb[Δa[Δb[mrg1[mrg2[agra agrb]]]]]]]:=ih _ _ H2.
+      exists Θa. exists Θb. exists (A.[σ] :L Δa). exists (_: Δb).
+      repeat split... }
+    { have[Θa[Θb[Δa[Δb[mrg1[mrg2[agra agrb]]]]]]]:=ih _ _ H2.
+      exists Θa. exists Θb. exists (_: Δa). exists (A.[σ] :L Δb).
+      repeat split... } }
+  { move=>Θ1 Γ1 Δ1 σ Γ2 Δ2 A s agr ih tyA Δa Δb mrg. inv mrg.
+    have[Θa[Θb[Δa[Δb[mrg1[mrg2[agra agrb]]]]]]]:=ih _ _ H2.
+    exists Θa. exists Θb. exists (_: Δa). exists (_: Δb).
+    repeat split... }
+  { move=>Θ1 Γ1 Δ1 σ Γ2 Δ2 A s agr ih tyA Δa Δb mrg. inv mrg.
+    have[Θa[Θb[Δa[Δb[mrg1[mrg2[agra agrb]]]]]]]:=ih _ _ H2.
+    exists Θa. exists Θb. exists Δa. exists Δb.
+    repeat split... }
+  { move=>Θa Θb Θ1 Γ1 Γ2 σ Δ1 Δ2 Δa Δb n A s k1 k2 mrg1 mrg2 agr ih tyn Δa' Δb' mrg'. inv mrg'.
+    { have[Θa'[Θb'[Δa'[Δb'[mrg1'[mrg2'[agra agrb]]]]]]]:=ih _ _ H2.
+      have[Θc[mrg1a mrg1b]]:=merge_splitL mrg1 mrg1'.
+      have[Δc[mrg2a mrg2b]]:=merge_splitL mrg2 mrg2'.
+      exists Θc. exists Θb'. exists Δc. exists Δb'.
       repeat split...
-      apply: dyn_agree_subst_wk1...
-      have[Δd[mrg3 mrg4]]:=merge_splitR mrg mrg'.
-      have e:=merge_pureR mrg3 k.
-      by subst. }
-    { have[Δa'[Δb'[mrg'[agra agrb]]]]:=ih _ _ H2.
-      have[Δc[mrg1 mrg2]]:=merge_splitL mrg mrg'.
-      exists Δc. exists Δb'.
+      have[Θd[mrg3 _]]:=merge_splitR mrg1 mrg1'.
+      have[Δd[mrg4 _]]:=merge_splitR mrg2 mrg2'.
+      have e:=merge_pureR mrg3 k1. subst.
+      have e:=merge_pureR mrg4 k2. subst.
+      apply: dyn_agree_subst_wk1. apply: k1. apply: k2.
+      apply: mrg3. apply: mrg4. apply: agrb. apply: tyn. }
+    { have[Θa'[Θb'[Δa'[Δb'[mrg1'[mrg2'[agra agrb]]]]]]]:=ih _ _ H2.
+      have[Θc[mrg1a mrg1b]]:=merge_splitL mrg1 mrg1'.
+      have[Δc[mrg2a mrg2b]]:=merge_splitL mrg2 mrg2'.
+      exists Θc. exists Θb'. exists Δc. exists Δb'.
       repeat split...
       apply: dyn_agree_subst_wk0...
       apply: dyn_sta_type... }
-    { have[Δa'[Δb'[mrg'[agra agrb]]]]:=ih _ _ H2.
-      have[Δc[mrg1 mrg2]]:=merge_splitR mrg mrg'.
-      exists Δa'. exists Δc.
+    { have[Θa'[Θb'[Δa'[Δb'[mrg1'[mrg2'[agra agrb]]]]]]]:=ih _ _ H2.
+      have[Θc[mrg1a mrg1b]]:=merge_splitR mrg1 mrg1'.
+      have[Δc[mrg2a mrg2b]]:=merge_splitR mrg2 mrg2'.
+      exists Θa'. exists Θc. exists Δa'. exists Δc.
       repeat split...
-      exact: merge_sym.
+      apply: merge_sym...
+      apply: merge_sym...
       apply: dyn_agree_subst_wk0...
       apply: dyn_sta_type... } }
-  { move=>Γ1 Δ1 σ Γ2 Δ2 A B s eq tyB1 tyB2 agr ih Δa Δb mrg. inv mrg.
-    have[Δa'[Δb'[mrg'[agra agrb]]]]:=ih _ _ (merge_null H2).
-    exists Δa'. exists Δb'... }
-  { move=>Γ1 Δ1 σ Γ2 Δ2 A B s eq tyB1 tyB2 agr ih Δa Δb mrg. inv mrg.
-    { have[Δa'[Δb'[mrg'[agra agrb]]]]:=ih _ _ (merge_left A H2).
-      exists Δa'. exists Δb'... }
-    { have[Δa'[Δb'[mrg'[agra agrb]]]]:=ih _ _ (merge_right1 A H2).
-      exists Δa'. exists Δb'... }
-    { have[Δa'[Δb'[mrg'[agra agrb]]]]:=ih _ _ (merge_right2 A H2).
-      exists Δa'. exists Δb'... } }
+  { move=>Θ1 Γ1 Δ1 σ Γ2 Δ2 A B s eq tyB1 tyB2 agr ih Δa Δb mrg. inv mrg.
+    have[Θa'[Θb'[Δa'[Δb'[mrg1'[mrg2'[agra agrb]]]]]]]:=ih _ _ (merge_null H2).
+    exists Θa'. exists Θb'. exists Δa'. exists Δb'... }
+  { move=>Θ1 Γ1 Δ1 σ Γ2 Δ2 A B s eq tyB1 tyB2 agr ih Δa Δb mrg. inv mrg.
+    { have[Θa'[Θb'[Δa'[Δb'[mrg1'[mrg2'[agra agrb]]]]]]]:=ih _ _ (merge_left A H2).
+      exists Θa'. exists Θb'... exists Δa'. exists Δb'... }
+    { have[Θa'[Θb'[Δa'[Δb'[mrg1'[mrg2'[agra agrb]]]]]]]:=ih _ _ (merge_right1 A H2).
+      exists Θa'. exists Θb'... exists Δa'. exists Δb'... }
+    { have[Θa'[Θb'[Δa'[Δb'[mrg1'[mrg2'[agra agrb]]]]]]]:=ih _ _ (merge_right2 A H2).
+      exists Θa'. exists Θb'... exists Δa'. exists Δb'... } }
 Qed.
 
-Lemma dyn_agree_subst_wf_nil Γ1 Δ1 σ : Γ1; Δ1 ⊢ σ ⊣ [::]; [::] → dyn_wf Γ1 Δ1.
+Lemma dyn_agree_subst_wf_nil Θ1 Γ1 Δ1 σ : Θ1 ; Γ1; Δ1 ⊢ σ ⊣ [::]; [::] → dyn_wf Γ1 Δ1.
 Proof with eauto using dyn_wf.
   move e1:(nil)=>Γ2.
   move e2:(nil)=>Δ2 agr.
   elim: agr e1 e2=>//{Γ1 Γ2 Δ1 Δ2 σ}...
 Qed.
 
-Lemma dyn_agree_subst_wf_ty Γ1 Γ2 Δ1 Δ2 A s σ :
-  Γ1; Δ1 ⊢ σ ⊣ (A :: Γ2); A :{s} Δ2 -> dyn_wf Γ2 Δ2 ->
-  (∀ Γ1 Δ1 σ, Γ1; Δ1 ⊢ σ ⊣ Γ2; Δ2 → dyn_wf Γ1 Δ1) ->
+Lemma dyn_agree_subst_wf_ty Θ1 Γ1 Γ2 Δ1 Δ2 A s σ :
+  Θ1 ; Γ1; Δ1 ⊢ σ ⊣ (A :: Γ2); A :{s} Δ2 -> dyn_wf Γ2 Δ2 ->
+  (∀ Θ1 Γ1 Δ1 σ, Θ1 ; Γ1; Δ1 ⊢ σ ⊣ Γ2; Δ2 → dyn_wf Γ1 Δ1) ->
   dyn_wf Γ1 Δ1.
 Proof with eauto using dyn_wf.
   move e1:(A :: Γ2)=>Γ0.
   move e2:(A :{s} Δ2)=>Δ0 agr.
-  elim: agr A Γ2 Δ2 s e1 e2=>//{Γ0 Δ0 Γ1 Δ1 σ}...
-  { move=>Γ1 Δ1 σ Γ2 Δ2 A s agr _ tyA A0 Γ0 Δ0 s0[e1 e2][_ e3 e4]wf h; subst.
+  elim: agr A Γ2 Δ2 s e1 e2=>//{Θ1 Γ0 Δ0 Γ1 Δ1 σ}...
+  { move=>Θ1 Γ1 Δ1 σ Γ2 Δ2 A s agr _ tyA A0 Γ0 Δ0 s0[e1 e2][_ e3 e4]wf h; subst.
     apply: dyn_wf_ty...
     replace (Sort s) with (Sort s).[σ] by eauto.
     apply: sta_substitution...
     apply: dyn_sta_agree_subst... }
-  { move=>Γ1 Γ2 σ Δ1 Δ2 Δa Δb n A s k mrg agr _ tyn A0 Γ0 Δ0 s0
+  { move=>Θa Θb Θ1 Γ1 Γ2 σ Δ1 Δ2 Δa Δb n A s k1 k2 mrg1 mrg2 agr _ tyn A0 Γ0 Δ0 s0
       [e1 e2][_ e3 e4]wf h; subst.
     apply: dyn_wf_merge... }
-  { move=>Γ1 Δ1 σ Γ2 Δ2 A B s eq tyB1 tyB2 agr ih A0 Γ0 Δ0 s0
+  { move=>Θ1 Γ1 Δ1 σ Γ2 Δ2 A B s eq tyB1 tyB2 agr ih A0 Γ0 Δ0 s0
       [e1 e2][_ e3 e4]wf h; subst... }
 Qed.
 
-Lemma dyn_agree_subst_wf_n Γ1 Γ2 Δ1 Δ2 A σ :
-  Γ1; Δ1 ⊢ σ ⊣ (A :: Γ2); _: Δ2 -> dyn_wf Γ2 Δ2 ->
-  (∀ Γ1 Δ1 σ, Γ1; Δ1 ⊢ σ ⊣ Γ2; Δ2 → dyn_wf Γ1 Δ1) ->
+Lemma dyn_agree_subst_wf_n Θ1 Γ1 Γ2 Δ1 Δ2 A σ :
+  Θ1 ; Γ1; Δ1 ⊢ σ ⊣ (A :: Γ2); _: Δ2 -> dyn_wf Γ2 Δ2 ->
+  (∀ Θ1 Γ1 Δ1 σ, Θ1 ; Γ1; Δ1 ⊢ σ ⊣ Γ2; Δ2 → dyn_wf Γ1 Δ1) ->
   dyn_wf Γ1 Δ1.
 Proof with eauto using dyn_wf.
   move e1:(A :: Γ2)=>Γ0.
   move e2:(_: Δ2)=>Δ0 agr.
-  elim: agr A Γ2 Δ2 e1 e2=>//{Γ0 Δ0 Γ1 Δ1 σ}...
-  { move=>Γ1 Δ1 σ Γ2 Δ2 A s agr _ tyA A0 Γ0 Δ0[e1 e2][e3]wf h; subst.
+  elim: agr A Γ2 Δ2 e1 e2=>//{Θ1 Γ0 Δ0 Γ1 Δ1 σ}...
+  { move=>Θ1 Γ1 Δ1 σ Γ2 Δ2 A s agr _ tyA A0 Γ0 Δ0[e1 e2][e3]wf h; subst.
     apply: dyn_wf_n...
     have:=sta_substitution tyA (dyn_sta_agree_subst agr).
     asimpl... }
-  { move=>Γ1 Δ1 σ Γ2 Δ2 n A agr ih tyn A0 Γ0 Δ0[e1 e2][e3]wf h; subst... }
-  { move=>Γ1 Δ1 σ Γ2 Δ2 A B s eq tyB1 tyB2 agr ih A0 Γ0 Δ0
+  { move=>Θ1 Γ1 Δ1 σ Γ2 Δ2 n A agr ih tyn A0 Γ0 Δ0[e1 e2][e3]wf h; subst... }
+  { move=>Θ1 Γ1 Δ1 σ Γ2 Δ2 A B s eq tyB1 tyB2 agr ih A0 Γ0 Δ0
       [e1 e2][e3]wf h; subst... }
 Qed.
 
-Lemma dyn_substitution Γ1 Γ2 m A Δ1 Δ2 σ :
-  Γ2 ; Δ2 ⊢ m : A -> Γ1 ; Δ1 ⊢ σ ⊣ Γ2 ; Δ2 -> Γ1 ; Δ1 ⊢ m.[σ] : A.[σ].
+Lemma dyn_substitution Θ1 Θ2 Θ Γ1 Γ2 m A Δ1 Δ2 σ :
+  Θ2 ; Γ2 ; Δ2 ⊢ m : A -> Θ1 ∘ Θ2 => Θ ->
+  Θ1 ; Γ1 ; Δ1 ⊢ σ ⊣ Γ2 ; Δ2 -> Θ ; Γ1 ; Δ1 ⊢ m.[σ] : A.[σ].
 Proof with eauto using dyn_agree_subst, dyn_agree_subst_key, dyn_type.
-  move=>ty. move:Γ2 Δ2 m A ty Γ1 Δ1 σ.
-  apply:(@dyn_type_mut _ (fun Γ2 Δ2 wf => forall Γ1 Δ1 σ, Γ1 ; Δ1 ⊢ σ ⊣ Γ2 ; Δ2 -> dyn_wf Γ1 Δ1)).
-  { move=>Γ Δ x s A wf h shs dhs Γ1 Δ1 σ agr. asimpl.
+  move=>ty. move:Θ2 Γ2 Δ2 m A ty Θ1 Θ Γ1 Δ1 σ.
+  apply:(@dyn_type_mut _ (fun Γ2 Δ2 wf => forall Θ1 Γ1 Δ1 σ, Θ1 ; Γ1 ; Δ1 ⊢ σ ⊣ Γ2 ; Δ2 -> dyn_wf Γ1 Δ1)).
+  { move=>Θ2 Γ Δ x s A emp wf ih shs dhs Θ1 Θ Γ1 Δ1 σ mrg agr. asimpl.
     apply: dyn_agree_subst_has... }
-  { move=>Γ Δ A B m s k tym ihm Γ1 Δ1 σ agr. asimpl.
-    have wf:=dyn_type_wf tym. inv wf.
-    apply: dyn_lam0... }
-  { move=>Γ Δ A B m s t k tym ihm Γ1 Δ1 σ agr. asimpl.
-    have wf:=dyn_type_wf tym. inv wf.
-    apply: dyn_lam1... }
-  { move=>Γ Δ A B m n s tym ihm tyn Γ1 Δ1 σ agr. asimpl.
-    replace B.[n.[σ] .: σ] with B.[up σ].[n.[σ]/] by autosubst.
-    have{}ihm:=ihm _ _ _ agr.
-    apply: dyn_app0...
-    have//:=sta_substitution tyn (dyn_sta_agree_subst agr). }
-  { move=>Γ Δ1 Δ2 Δ A B m n s mrg tym ihm tyn ihn Γ1 Δ0 σ agr. asimpl.
-    replace B.[n.[σ] .: σ] with B.[up σ].[n.[σ]/] by autosubst.
-    have[Δa[Δb[mrg0[agra agrb]]]]:=dyn_agree_subst_merge agr mrg.
-    have{}ihm:=ihm _ _ _ agra.
-    have{}ihn:=ihn _ _ _ agrb.
-    apply: dyn_app1... }
-  { move=>Γ Δ A B m s eq tym ihm tyB Γ1 Δ1 σ agr.
-    apply: dyn_conv.
-    apply: sta_conv_subst...
-    apply: ihm...
-    have:=sta_substitution tyB (dyn_sta_agree_subst agr).
-    asimpl... }
-  { exact: dyn_agree_subst_wf_nil. }
-  { move=>Γ Δ A s wf h tyA Γ1 Δ1 σ agr.
-    apply: dyn_agree_subst_wf_ty... }
-  { move=>Γ Δ A s wf ih tyA Γ1 Δ1 σ agr.
-    apply: dyn_agree_subst_wf_n... }
-Qed.
+Admitted.
+(*   { move=>Γ Δ A B m s k tym ihm Γ1 Δ1 σ agr. asimpl. *)
+(*     have wf:=dyn_type_wf tym. inv wf. *)
+(*     apply: dyn_lam0... } *)
+(*   { move=>Γ Δ A B m s t k tym ihm Γ1 Δ1 σ agr. asimpl. *)
+(*     have wf:=dyn_type_wf tym. inv wf. *)
+(*     apply: dyn_lam1... } *)
+(*   { move=>Γ Δ A B m n s tym ihm tyn Γ1 Δ1 σ agr. asimpl. *)
+(*     replace B.[n.[σ] .: σ] with B.[up σ].[n.[σ]/] by autosubst. *)
+(*     have{}ihm:=ihm _ _ _ agr. *)
+(*     apply: dyn_app0... *)
+(*     have//:=sta_substitution tyn (dyn_sta_agree_subst agr). } *)
+(*   { move=>Γ Δ1 Δ2 Δ A B m n s mrg tym ihm tyn ihn Γ1 Δ0 σ agr. asimpl. *)
+(*     replace B.[n.[σ] .: σ] with B.[up σ].[n.[σ]/] by autosubst. *)
+(*     have[Δa[Δb[mrg0[agra agrb]]]]:=dyn_agree_subst_merge agr mrg. *)
+(*     have{}ihm:=ihm _ _ _ agra. *)
+(*     have{}ihn:=ihn _ _ _ agrb. *)
+(*     apply: dyn_app1... } *)
+(*   { move=>Γ Δ A B m s eq tym ihm tyB Γ1 Δ1 σ agr. *)
+(*     apply: dyn_conv. *)
+(*     apply: sta_conv_subst... *)
+(*     apply: ihm... *)
+(*     have:=sta_substitution tyB (dyn_sta_agree_subst agr). *)
+(*     asimpl... } *)
+(*   { exact: dyn_agree_subst_wf_nil. } *)
+(*   { move=>Γ Δ A s wf h tyA Γ1 Δ1 σ agr. *)
+(*     apply: dyn_agree_subst_wf_ty... } *)
+(*   { move=>Γ Δ A s wf ih tyA Γ1 Δ1 σ agr. *)
+(*     apply: dyn_agree_subst_wf_n... } *)
+(* Qed. *)
 
-Lemma dyn_substitution_wf Γ1 Γ2 Δ1 Δ2 σ :
-  dyn_wf Γ2 Δ2 -> Γ1 ; Δ1 ⊢ σ ⊣ Γ2 ; Δ2 -> dyn_wf Γ1 Δ1.
-Proof with eauto using dyn_wf.
-  move=>wf. elim: wf Γ1 Δ1 σ=>{Γ2 Δ2}.
-  { move=>*. apply: dyn_agree_subst_wf_nil... }
-  { move=>*. apply: dyn_agree_subst_wf_ty... }
-  { move=>*. apply: dyn_agree_subst_wf_n... }
-Qed.
+(* Lemma dyn_substitution_wf Γ1 Γ2 Δ1 Δ2 σ : *)
+(*   dyn_wf Γ2 Δ2 -> Γ1 ; Δ1 ⊢ σ ⊣ Γ2 ; Δ2 -> dyn_wf Γ1 Δ1. *)
+(* Proof with eauto using dyn_wf. *)
+(*   move=>wf. elim: wf Γ1 Δ1 σ=>{Γ2 Δ2}. *)
+(*   { move=>*. apply: dyn_agree_subst_wf_nil... } *)
+(*   { move=>*. apply: dyn_agree_subst_wf_ty... } *)
+(*   { move=>*. apply: dyn_agree_subst_wf_n... } *)
+(* Qed. *)
 
-Lemma dyn_subst0 Γ Δ m n A B :
-  (A :: Γ) ; _: Δ ⊢ m : B -> Γ ⊢ n : A -> Γ ; Δ ⊢ m.[n/] : B.[n/].
+Lemma dyn_subst0 Θ Γ Δ m n A B :
+  Θ ; (A :: Γ) ; _: Δ ⊢ m : B -> Γ ⊢ n : A -> Θ ; Γ ; Δ ⊢ m.[n/] : B.[n/].
 Proof with eauto using dyn_agree_subst_refl.
   move=>tym tyn.
   have wf:=dyn_type_wf tym. inv wf.
+  have[Θ0[emp mrg]]:=dyn_type_empty tym.
   apply: dyn_substitution...
   apply: dyn_agree_subst_wk0...
   by asimpl.
 Qed.
 
-Lemma dyn_subst1 Γ Δ1 Δ2 Δ m n A B s :
+Lemma dyn_subst1 Θ1 Θ2 Θ Γ Δ1 Δ2 Δ m n A B s :
+  Θ2 ▷ s -> Θ1 ∘ Θ2 => Θ ->
   Δ2 ▷ s -> Δ1 ∘ Δ2 => Δ ->
-  (A :: Γ) ; A :{s} Δ1 ⊢ m : B -> Γ ; Δ2 ⊢ n : A -> Γ ; Δ ⊢ m.[n/] : B.[n/].
+  Θ1 ; (A :: Γ) ; A :{s} Δ1 ⊢ m : B ->
+  Θ2 ; Γ ; Δ2 ⊢ n : A ->
+  Θ ; Γ ; Δ ⊢ m.[n/] : B.[n/].
 Proof with eauto using dyn_agree_subst_refl.
-  move=>k mrg tym tyn.
+  move=>k1 mrg1 k2 mrg2 tym tyn.
   have wf:=dyn_type_wf tym. inv wf.
+  have[Θ0[emp mrg]]:=dyn_type_empty tyn.
   apply: dyn_substitution...
-  apply: dyn_agree_subst_wk1...
+  apply: merge_sym...
+  apply: dyn_agree_subst_wk1.
+  apply: k1. apply: k2.
+  apply: mrg.
+  apply: mrg2.
+  apply: dyn_agree_subst_refl...
   by asimpl.
 Qed.
 
