coq_session/dyn_valid.v
@@ -6,14 +6,14 @@ Set Implicit Arguments.
 Unset Strict Implicit.
 Unset Printing Implicit Defensive.
 
-Lemma dyn_sta_type Γ Δ m A : Γ ; Δ ⊢ m : A -> Γ ⊢ m : A.
+Lemma dyn_sta_type Θ Γ Δ m A : Θ ; Γ ; Δ ⊢ m : A -> Γ ⊢ m : A.
 Proof with eauto using sta_type, sta_wf.
   move:Γ Δ m A.
   apply:(@dyn_type_mut _ (fun Γ Δ wf => sta_wf Γ))...
-  Unshelve. all: eauto.
+  Unshelve. all: eauto using bool.
 Qed.
 
-Theorem dyn_valid Γ Δ m A : Γ ; Δ ⊢ m : A -> exists s, Γ ⊢ A : Sort s.
+Theorem dyn_valid Θ Γ Δ m A : Θ ; Γ ; Δ ⊢ m : A -> exists s, Γ ⊢ A : Sort s.
 Proof.
   move=>ty.
   apply: sta_valid.
